src/Crypto/HKDF/HMAC.dfy
@@ -8,61 +8,44 @@ module {:extern "HMAC"} HMAC {
 
   datatype {:extern "CipherParameters"} CipherParameters = KeyParameter(key: seq<uint8>)
 
+  // Hash length in octets (bytes), e.g. GetHashLength(SHA256) ==> 256 bits = 32 bytes ==> n = 32
+  function method GetHashLength(algorithm: KeyDerivationAlgorithm): (n: int32)
+    requires algorithm != IDENTITY
+    ensures algorithm == HKDF_WITH_SHA_256 ==> n == 32
+    ensures algorithm == HKDF_WITH_SHA_384 ==> n == 48
+  {
+    match algorithm {
+      case HKDF_WITH_SHA_256 => 32
+      case HKDF_WITH_SHA_384 => 48
+    }
+  }
+
   class {:extern "HMac"} HMac {
 
-    const algorithm: KeyDerivationAlgorithm
     ghost var initialized: Option<seq<uint8>>
-    ghost var InputSoFar: seq<uint8>
 
     constructor {:extern} (algorithm: KeyDerivationAlgorithm)
       requires algorithm != IDENTITY
-      ensures this.algorithm == algorithm
 
-    function method {:extern "GetMacSize"} getMacSize(): int32
-      requires algorithm != IDENTITY
-      ensures getMacSize() == HashLength(algorithm)
+    predicate {:axiom} ValidKey(key: seq<uint8>)
 
-    predicate {:axiom} validKey(key: seq<uint8>)
-
-    method {:extern "Init"} init(params: CipherParameters)
-      // The documentation says it can throw "InvalidKeyException - if the given key is inappropriate for
-      // initializing this MAC", which I have interpreted to mean the following precondition:
+    method {:extern "Init"} Init(params: CipherParameters)
       requires params.KeyParameter?
-      modifies this
       ensures
         var key := match params case KeyParameter(key) => key;
-        match initialized { case Some(k) => validKey(k) && key == k case None => false }
-      ensures InputSoFar == []
+        match initialized { case Some(k) => ValidKey(k) && key == k case None => false }
 
-    method {:extern "Update"} updateSingle(input: uint8)
+    method {:extern "Update"} UpdateSingle(input: uint8)
       requires initialized.Some?
-      modifies this
-      ensures unchanged(`initialized)
-      ensures InputSoFar == old(InputSoFar) + [input]
 
-    method {:extern "BlockUpdate"} update(input: seq<uint8>, inOff: int32, len: int32)
+    method {:extern "BlockUpdate"} Update(input: seq<uint8>, inOff: int32, len: int32)
       requires initialized.Some?
       requires inOff >= 0
       requires len >= 0
       requires |input| < INT32_MAX_LIMIT
       requires inOff as int + len as int <= |input|
-      modifies `InputSoFar
-      ensures InputSoFar == old(InputSoFar) + input[inOff..(inOff + len)]
 
-    method {:extern "GetResult"} getResult() returns (s: seq<uint8>)
+    method {:extern "GetResult"} GetResult() returns (s: seq<uint8>)
       requires initialized.Some?
-      requires algorithm != IDENTITY
-      modifies `InputSoFar
-      ensures InputSoFar == []
-      ensures |s| == HashLength(algorithm) as int
-
-    method updateAll(input: seq<uint8>)
-      requires initialized.Some?
-      requires |input| < INT32_MAX_LIMIT
-      modifies `InputSoFar
-      ensures InputSoFar == old(InputSoFar) + input
-    {
-      update(input, 0, |input| as int32);
-    }
   }
 }
