src/Crypto/HKDF/HKDF.dfy
@@ -27,53 +27,55 @@ module HKDF {
   import opened StandardLibrary
   import opened UInt = StandardLibrary.UInt
 
-  method extract(algorithm: KeyDerivationAlgorithm, hmac: HMac, salt: seq<uint8>, ikm: seq<uint8>) returns (prk: seq<uint8>)
-    requires hmac.algorithm == algorithm && |salt| != 0
+  method Extract(algorithm: KeyDerivationAlgorithm, hmac: HMac, salt: seq<uint8>, ikm: seq<uint8>) returns (prk: seq<uint8>)
+    requires |salt| != 0
     requires algorithm != IDENTITY
     requires |ikm| < INT32_MAX_LIMIT
     modifies hmac
-    ensures |prk| > 0 && HashLength(algorithm) as int <= |prk|
+    ensures |prk| > 0 && GetHashLength(algorithm) as int <= |prk|
   {
     var params: CipherParameters := KeyParameter(salt);
-    hmac.init(params);
-    assert hmac.InputSoFar + ikm == ikm;
-    hmac.updateAll(ikm);
-    prk := hmac.getResult();
+
+    hmac.Init(params);
+    hmac.Update(ikm, 0, |ikm| as int32);
+    prk := hmac.GetResult();
     return prk;
   }
 
-  method expand(algorithm: KeyDerivationAlgorithm, hmac: HMac, prk: seq<uint8>, info: seq<uint8>, n: int) returns (a: seq<uint8>)
-    requires hmac.algorithm == algorithm && 1 <= n <= 255
+  method Expand(algorithm: KeyDerivationAlgorithm, hmac: HMac, prk: seq<uint8>, info: seq<uint8>, n: int) returns (a: seq<uint8>)
+    requires 1 <= n <= 255
     requires algorithm != IDENTITY
-    requires 0 != |prk| && HashLength(algorithm) as int <= |prk|
+    requires 0 != |prk| && GetHashLength(algorithm) as int <= |prk|
     requires |info| < INT32_MAX_LIMIT
     modifies hmac
-    ensures |a| == n * hmac.getMacSize() as int;
+    ensures |a| == n * GetHashLength(algorithm) as int;
   {
     var params: CipherParameters := KeyParameter(prk);
-    hmac.init(params);
-    ghost var gKey := hmac.initialized.get;
+    hmac.Init(params);
 
-    hmac.updateAll(info);
-    hmac.updateSingle(1 as uint8);
-    var TiSeq := hmac.getResult();
+    var hashLength := GetHashLength(algorithm);
+    hmac.Update(info, 0, |info| as int32);
+    hmac.UpdateSingle(1 as uint8);
+    var TiSeq := hmac.GetResult();
     a := TiSeq;
 
     var i := 1;
     while i < n
       invariant 1 <= i <= n
-      invariant |TiSeq| == hmac.getMacSize() as int
-      invariant hmac.getMacSize() as int <= |prk|
-      invariant |a| == i * hmac.getMacSize() as int;
-      invariant hmac.initialized.Some? && hmac.initialized.get == gKey
-      invariant hmac.InputSoFar == []
+      invariant |TiSeq| == hashLength as int
+      invariant hashLength as int <= |prk|
+      invariant |a| == i * hashLength as int;
+      invariant hmac.initialized.Some?
     {
-      hmac.updateAll(TiSeq);
-      hmac.updateAll(info);
-      hmac.updateSingle((i+1) as uint8);
+      hmac.Update(TiSeq, 0, |TiSeq| as int32);
+      hmac.Update(info, 0, |info| as int32);
+      hmac.UpdateSingle((i+1) as uint8);
       assert (i+1) <= 255;
-      assert hmac.InputSoFar == TiSeq + info + [((i+1) as uint8)];
-      TiSeq := hmac.getResult();
+
+      TiSeq := hmac.GetResult();
+      var offset := i * hashLength as int;
+      assert offset < n * hashLength as int;
+      assert offset < |a|;
       a := a + TiSeq;
       i := i + 1;
     }
@@ -82,9 +84,9 @@ module HKDF {
   /**
    * The RFC 5869 KDF. Outputs L bytes of output key material.
    **/
-  method hkdf(algorithm: KeyDerivationAlgorithm, salt: Option<seq<uint8>>, ikm: seq<uint8>, info: seq<uint8>, L: int) returns (okm: seq<uint8>)
+  method Hkdf(algorithm: KeyDerivationAlgorithm, salt: Option<seq<uint8>>, ikm: seq<uint8>, info: seq<uint8>, L: int) returns (okm: seq<uint8>)
     requires algorithm != IDENTITY
-    requires 0 <= L <= 255 * HashLength(algorithm) as int
+    requires 0 <= L <= 255 * GetHashLength(algorithm) as int
     requires salt.None? || |salt.get| != 0
     requires |info| < INT32_MAX_LIMIT
     requires |ikm| < INT32_MAX_LIMIT
@@ -95,19 +97,20 @@ module HKDF {
     }
     var hmac := new HMac(algorithm);
 
+    var hashLength := GetHashLength(algorithm);
     var saltNonEmpty: seq<uint8>;
     match salt {
       case None =>
-        saltNonEmpty := seq(hmac.getMacSize() as int, _ => 0);
+        saltNonEmpty := seq(hashLength as int, _ => 0);
       case Some(s) =>
         saltNonEmpty := s;
     }
-    assert saltNonEmpty == if salt.None? then Fill(0, hmac.getMacSize() as int) else salt.get; // nfv
+    assert saltNonEmpty == if salt.None? then Fill(0, hashLength as int) else salt.get; // nfv
 
-    var n := 1 + (L-1) / hmac.getMacSize() as int;  // note, since L and HMAC_SIZE are strictly positive, this gives the same result in Java as in Dafny
-    assert n * hmac.getMacSize() as int >= L;
-    var prk := extract(algorithm, hmac, saltNonEmpty, ikm);
-    okm := expand(algorithm, hmac, prk, info, n);
+    var n := 1 + (L-1) / hashLength as int;  // note, since L and HMAC_SIZE are strictly positive, this gives the same result in Java as in Dafny
+    assert n * hashLength as int >= L;
+    var prk := Extract(algorithm, hmac, saltNonEmpty, ikm);
+    okm := Expand(algorithm, hmac, prk, info, n);
 
     // if necessary, trim padding
     if |okm| > L {
